examples/miniML/hol2miniml/okasaki-examples/BatchedQueueScript.sml
@@ -43,22 +43,23 @@ val empty_thm = prove(
 
 val is_empty_thm = prove(
   ``!q xs. queue_inv xs q ==> (is_empty q = (xs = []))``,
-  Cases THEN Cases_on `l` THEN EVAL_TAC THEN SRW_TAC [] []
-  THEN FULL_SIMP_TAC std_ss [REVERSE_DEF]);
+  Cases THEN Cases_on `l` THEN EVAL_TAC THEN SRW_TAC [] [REV_DEF]);
 
 val snoc_thm = prove(
   ``!q xs x. queue_inv xs q ==> queue_inv (xs ++ [x]) (snoc q x)``,
-  Cases THEN Cases_on `l` THEN EVAL_TAC THEN SRW_TAC [] []);
+  Cases THEN Cases_on `l` THEN FULL_SIMP_TAC (srw_ss())
+    [queue_inv_def,snoc_def,REVERSE_DEF,checkf_def,APPEND]);
 
 val head_thm = prove(
   ``!q x xs. queue_inv (x::xs) q ==> (head q = x)``,
-  Cases THEN Cases_on `l` THEN EVAL_TAC THEN SRW_TAC [] []
-  THEN FULL_SIMP_TAC (srw_ss()) [REVERSE_DEF]);
+  Cases THEN Cases_on `l` THEN FULL_SIMP_TAC (srw_ss())
+    [queue_inv_def,head_def,REVERSE_DEF,checkf_def,APPEND]
+  THEN REPEAT STRIP_TAC THEN FULL_SIMP_TAC (srw_ss()) []);
 
 val tail_thm = prove(
   ``!q x xs. queue_inv (x::xs) q ==> queue_inv xs (tail q)``,
   Cases THEN Cases_on `l` THEN EVAL_TAC THEN SRW_TAC [] []
   THEN TRY (Cases_on `t`) THEN EVAL_TAC
-  THEN FULL_SIMP_TAC (srw_ss()) [REVERSE_DEF]);
+  THEN FULL_SIMP_TAC (srw_ss()) [REVERSE_DEF,REV_DEF]);
 
 val _ = export_theory();
