examples/miniML/hol2miniml/okasaki-examples/RealTimeQueueScript.sml
@@ -50,7 +50,8 @@ val empty_thm = prove(
 
 val is_empty_thm = prove(
   ``!q xs. queue_inv xs q ==> (is_empty q = (xs = []))``,
-  Cases THEN Cases_on `l` THEN EVAL_TAC THEN SRW_TAC [] [LENGTH_NIL]);
+  Cases THEN Cases_on `l`
+  THEN SRW_TAC [] [LENGTH_NIL,queue_inv_def,is_empty_def,prop_def,LENGTH]);
 
 val rotate_thm = prove(
   ``!f r s.
@@ -66,24 +67,28 @@ val rotate_thm = prove(
 val exec_thm = prove(
   ``prop 1 xs (QUEUE f r s) ==>
     queue_inv xs (exec (QUEUE f r s))``,
-  Cases_on `s` THEN EVAL_TAC THEN FULL_SIMP_TAC std_ss [rotate_thm,APPEND_NIL]
+  Cases_on `s` THEN FULL_SIMP_TAC (srw_ss())
+    [rotate_thm,exec_def,LET_DEF,prop_def,queue_inv_def]
   THEN REPEAT STRIP_TAC THEN DECIDE_TAC);
 
 val snoc_thm = prove(
   ``!q xs x. queue_inv xs q ==> queue_inv (xs ++ [x]) (snoc q x)``,
-  Cases THEN EVAL_TAC THEN REPEAT STRIP_TAC
-  THEN MATCH_MP_TAC exec_thm THEN EVAL_TAC
-  THEN FULL_SIMP_TAC (srw_ss()) [] THEN DECIDE_TAC);
+  Cases THEN FULL_SIMP_TAC (srw_ss())
+    [rotate_thm,LET_DEF,prop_def,queue_inv_def,snoc_def]
+  THEN REPEAT STRIP_TAC THEN MATCH_MP_TAC exec_thm
+  THEN FULL_SIMP_TAC (srw_ss()) [prop_def] THEN DECIDE_TAC);
 
 val head_thm = prove(
   ``!q x xs. queue_inv (x::xs) q ==> (head q = x)``,
-  Cases THEN Cases_on `l` THEN EVAL_TAC THEN SRW_TAC [] []
-  THEN FULL_SIMP_TAC (srw_ss()) [LENGTH_NIL,REVERSE_DEF]);
+  Cases THEN Cases_on `l` THEN FULL_SIMP_TAC (srw_ss())
+    [rotate_thm,LET_DEF,prop_def,queue_inv_def,head_def]
+  THEN SRW_TAC [] [] THEN FULL_SIMP_TAC (srw_ss()) [LENGTH_NIL,REVERSE_DEF]);
 
 val tail_thm = prove(
   ``!q x xs. queue_inv (x::xs) q ==> queue_inv xs (tail q)``,
-  Cases THEN Cases_on `l` THEN EVAL_TAC THEN SRW_TAC [] []
-  THEN1 (FULL_SIMP_TAC (srw_ss()) [LENGTH_NIL,REVERSE_DEF])
+  Cases THEN Cases_on `l` THEN FULL_SIMP_TAC (srw_ss())
+    [rotate_thm,LET_DEF,prop_def,queue_inv_def,tail_def]
+  THEN SRW_TAC [] [] THEN FULL_SIMP_TAC (srw_ss()) [LENGTH_NIL,REVERSE_DEF]
   THEN MATCH_MP_TAC exec_thm THEN EVAL_TAC THEN DECIDE_TAC);
 
 val _ = export_theory();
